More work toward sketching out the type inference proof
Got a simple lemma about infer_e to go through (that the next
unification variable to be allocated does not decrease).  So at least
the basic infrastructure should be in place for getting rid of all of
the monadic aspects if infer_e.

type_checker/inferScript.sml
@@ -64,7 +64,7 @@ val failwith_def = Define `
 (failwith : α -> (β, γ, α) M) msg = (\s. (Failure msg, s))`;
 
 val guard_def = Define `
-guard P msg = if P then failwith msg else return ()`;
+guard P msg = if P then return () else failwith msg`;
 
 val read_def = Define `
 (read : (α, α, β) M) =
@@ -128,7 +128,9 @@ val add_constraints_def = Define `
   do () <- add_constraint t1 t2;
      () <- add_constraints ts1 ts2;
      return ()
-  od)`;
+  od) ∧
+(add_constraints _ _ =
+  failwith "Bad call to add_constraints")`;
 
 val get_next_uvar_def = Define `
 get_next_uvar =
