type_checker/inferSoundScript.sml
@@ -12,6 +12,12 @@ val count_add1 = Q.prove (
 `!n. count (n + 1) = n INSERT count n`,
 metis_tac [COUNT_SUC, arithmeticTheory.ADD1]);
 
+val st_ex_return_success = Q.prove (
+`!v st v' st'.
+  (st_ex_return v st = (Success v', st')) =
+  ((v = v') ∧ (st = st'))`,
+rw [st_ex_return_def]);
+
 val st_ex_bind_success = Q.prove (
 `!f g st st' v. 
  (st_ex_bind f g st = (Success v, st')) =
@@ -30,6 +36,33 @@ val fresh_uvar_success = Q.prove (
 rw [fresh_uvar_def] >>
 metis_tac []);
 
+val stupid_record_thing = Q.prove (
+`(!st. (st with next_uvar := st.next_uvar) = st) ∧
+ (!st. (st with subst := st.subst) = st)`,
+cheat);
+
+val count_list_sub1 = Q.prove (
+`!n. (n ≠ 0) ⇒ (COUNT_LIST n = 0::MAP SUC (COUNT_LIST (n - 1)))`,
+induct_on `n` >>
+ONCE_REWRITE_TAC [rich_listTheory.COUNT_LIST_def] >>
+fs []);
+
+val n_fresh_uvar_success = Q.prove (
+`!n st ts st'. 
+  (n_fresh_uvar n st = (Success ts, st')) =
+  ((ts = MAP (\n. Infer_Tuvar (st.next_uvar + n)) (COUNT_LIST n)) ∧
+   (st' = st with next_uvar := st.next_uvar + n))`,
+ho_match_mp_tac n_fresh_uvar_ind >>
+rw [] >>
+rw [st_ex_return_success, Once n_fresh_uvar_def, rich_listTheory.COUNT_LIST_SNOC,
+    st_ex_bind_success, fresh_uvar_success, stupid_record_thing] >-
+metis_tac [] >>
+fs [] >>
+srw_tac [ARITH_ss] [] >>
+rw [count_list_sub1, MAP_APPEND, MAP_MAP_o, combinTheory.o_DEF] >>
+eq_tac >>
+srw_tac [ARITH_ss] [arithmeticTheory.ADD1]);
+
 val apply_subst_success = Q.prove (
 `!t1 st1 t2 st2.
   (apply_subst t1 st1 = (Success t2, st2))
@@ -39,6 +72,135 @@ val apply_subst_success = Q.prove (
 rw [LET_THM, apply_subst_def] >>
 eq_tac >>
 rw []);
+
+val add_constraint_success = Q.prove (
+`!t1 t2 st st' x.
+  (add_constraint t1 t2 st = (Success x, st'))
+  =
+  ((x = ()) ∧ (?s. (t_unify st.subst t1 t2 = SOME s) ∧ (st' = st with subst := s)))`,
+rw [add_constraint_def] >>
+full_case_tac >>
+metis_tac []);
+
+val pure_add_constraints_def = Define `
+(pure_add_constraints [s] [] [] = T) ∧
+(pure_add_constraints (s1::s2::rest) (t1::ts1) (t2::ts2) = 
+  (t_unify s1 t1 t2 = SOME s2) ∧
+  pure_add_constraints (s2::rest) ts1 ts2) ∧
+(pure_add_constraints _ _ _ = F)`;
+
+val add_constraints_success = Q.prove (
+`!ts1 ts2 st st' x.
+  (add_constraints ts1 ts2 st = (Success x, st'))
+  =
+  ((x = ()) ∧ (?s. pure_add_constraints s ts1 ts2 ∧ (HD s = st.subst) ∧ (st' = st with subst := LAST s)))`,
+ho_match_mp_tac add_constraints_ind >>
+rw [add_constraints_def, pure_add_constraints_def, st_ex_return_success,
+    failwith_def, st_ex_bind_success, add_constraint_success] >>
+TRY (cases_on `x`) >>
+rw [pure_add_constraints_def] >|
+[eq_tac >>
+     rw [] >|
+     [qexists_tac `[st.subst]` >>
+          rw [pure_add_constraints_def, stupid_record_thing],
+      cases_on `s` >>
+          fs [pure_add_constraints_def] >>
+          cases_on `t` >>
+          fs [pure_add_constraints_def, stupid_record_thing]],
+ eq_tac >>
+     rw [] >|
+     [qexists_tac `st.subst::s'` >>
+          rw [] >>
+          cases_on `s'` >>
+          fs [pure_add_constraints_def],
+      cases_on `s` >>
+          fs [pure_add_constraints_def] >>
+          cases_on `t` >>
+          fs [pure_add_constraints_def] >>
+          rw [] >>
+          qexists_tac `h'::t'` >>
+          rw []],
+ cases_on `s` >>
+     fs [pure_add_constraints_def],
+ cases_on `s` >>
+     fs [pure_add_constraints_def]]);
+
+val failwith_success = Q.prove (
+`!m st v st'. (failwith m st = (Success v, st')) = F`,
+rw [failwith_def]);
+
+val lookup_st_ex_success = Q.prove (
+`!pr x l st v st'. 
+  (lookup_st_ex pr x l st = (Success v, st'))
+  =
+  ((lookup x l = SOME v) ∧ (st = st'))`,
+ho_match_mp_tac lookup_st_ex_ind >>
+rw [lookup_st_ex_def, lookup_def, failwith_def, st_ex_return_success]);
+
+val constrain_uop_success = Q.prove (
+`!uop t st v st'.
+  (constrain_uop uop t st = (Success v, st'))
+  =
+  (((uop = Opref) ∧ (st = st') ∧ (v = Infer_Tapp [t] TC_ref)) ∨
+   ((uop = Opderef) ∧ 
+    (?uvar st''. ((fresh_uvar : ((num |-> infer_t) elab_st, infer_t, string) M) st = (Success uvar, st'')) ∧
+                 (v = uvar) ∧
+                 (add_constraint t (Infer_Tapp [uvar] TC_ref) st'' = (Success (), st')))))`,
+rw [constrain_uop_def] >>
+full_case_tac >>
+rw [st_ex_return_success, st_ex_bind_success, oneTheory.one] >>
+metis_tac []);
+
+val op_case_expand = Q.prove (
+`!f1 f2 f3 f4 f5 op st v st'.
+  ((case op of
+       Opn opn => f1
+     | Opb opb => f2
+     | Equality => f3
+     | Opapp => f4
+     | Opassign => f5) st
+   = (Success v, st'))
+  =
+  ((?opn. (op = Opn opn) ∧ (f1 st = (Success v, st'))) ∨
+   (?opb. (op = Opb opb) ∧ (f2 st = (Success v, st'))) ∨
+   ((op = Equality) ∧ (f3 st = (Success v, st'))) ∨
+   ((op = Opapp) ∧ (f4 st = (Success v, st'))) ∨
+   ((op = Opassign) ∧ (f5 st = (Success v, st'))))`,
+rw [] >>
+cases_on `op` >>
+rw []);
+
+val constrain_op_success = 
+  SIMP_CONV (srw_ss()) [constrain_op_def, op_case_expand, st_ex_bind_success,
+                        st_ex_return_success, add_constraint_success]
+  ``(constrain_op op t1 t2 st = (Success v, st'))``
+
+val get_next_uvar_success = Q.prove (
+`!st v st'. 
+  (get_next_uvar st = (Success v, st')) 
+  =
+  ((v = st.next_uvar) ∧ (st = st'))`,
+rw [get_next_uvar_def] >>
+metis_tac []);
+
+val apply_subst_list_success =
+  SIMP_CONV (srw_ss()) [apply_subst_list_def, LET_THM]
+  ``(apply_subst_list ts st = (Success v, st'))``
+
+val guard_success = Q.prove (
+`∀P m st v st'.
+  (guard P m st = (Success v, st'))
+  =
+  (P ∧ (v = ()) ∧ (st = st'))`,
+rw [guard_def, st_ex_return_def, failwith_def] >>
+metis_tac []);
+
+val success_eqns = 
+  LIST_CONJ [st_ex_return_success, st_ex_bind_success, fresh_uvar_success,
+             apply_subst_success, add_constraint_success, lookup_st_ex_success,
+             n_fresh_uvar_success, failwith_success, add_constraints_success,
+             constrain_uop_success, constrain_op_success, oneTheory.one,
+             get_next_uvar_success, apply_subst_list_success, guard_success];
 
 val check_t_def = tDefine "check_t" `
 (check_t n uvars (Infer_Tuvar v) = v ∈ uvars) ∧
@@ -51,6 +213,10 @@ val check_t_def = tDefine "check_t" `
  rw [infer_t_size_def] >>
  res_tac >>
  decide_tac);
+
+val check_env_def = Define `
+check_env uvars env =
+  EVERY (\(x, (tvs,t)). check_t tvs uvars t)  env`;
 
 val check_menv_def = Define `
 check_menv menv =
@@ -95,6 +261,13 @@ sub_ext dom num_tvs sub ext =
   (FDOM ext = dom DIFF FDOM sub) ∧
   (!t. t ∈ FRANGE ext ⇒ check_t num_tvs {} t)`;
 
+val remove_pair_lem = Q.prove (
+`(!f v. (\(x,y). f x y) v = f (FST v) (SND v)) ∧
+ (!f v. (\(x,y,z). f x y z) v = f (FST v) (FST (SND v)) (SND (SND v)))`,
+rw [] >>
+PairCases_on `v` >>
+rw []);
+
 val check_convert_freevars = Q.prove (
 `(!tvs uvs t. check_t tvs uvs t ⇒ (uvs = {}) ⇒ check_freevars tvs [] (convert_t t))`,
 ho_match_mp_tac (fetch "-" "check_t_ind") >>
@@ -102,7 +275,52 @@ rw [check_freevars_def, check_t_def, convert_t_def] >>
 fs [EVERY_MEM, MEM_MAP] >>
 metis_tac []);
 
-(*
+val infer_p_next_uvar_mono = Q.prove (
+`(!cenv p st t env st'.
+    (infer_p cenv p st = (Success (t,env), st'))
+    ⇒
+    st.next_uvar ≤ st'.next_uvar) ∧
+ (!cenv ps st ts env st'.
+    (infer_ps cenv ps st = (Success (ts,env), st'))
+    ⇒
+    st.next_uvar ≤ st'.next_uvar)`,
+ho_match_mp_tac infer_p_ind >>
+rw [infer_p_def, success_eqns, remove_pair_lem, GSYM FORALL_PROD] >>
+rw [] >>
+res_tac >>
+fs [] >>
+metis_tac [DECIDE ``!(x:num) y z. x ≤ y ⇒ x ≤ y + z``,
+           arithmeticTheory.LESS_EQ_TRANS]);
+
+val infer_e_next_uvar_mono = Q.prove (
+`(!menv cenv env e st st' t.
+    (infer_e menv cenv env e st = (Success t, st'))
+    ⇒
+    st.next_uvar ≤ st'.next_uvar) ∧
+ (!menv cenv env es st st' ts.
+    (infer_es menv cenv env es st = (Success ts, st'))
+    ⇒
+    st.next_uvar ≤ st'.next_uvar) ∧
+ (!menv cenv env pes t1 t2 st st'.
+    (infer_pes menv cenv env pes t1 t2 st = (Success (), st'))
+    ⇒
+    st.next_uvar ≤ st'.next_uvar) ∧
+ (!menv cenv env funs st st'.
+    (infer_funs menv cenv env funs st = (Success (), st'))
+    ⇒
+    st.next_uvar ≤ st'.next_uvar)`,
+ho_match_mp_tac infer_e_ind >>
+rw [infer_e_def, success_eqns, remove_pair_lem, GSYM FORALL_PROD] >>
+rw [] >>
+res_tac >>
+fs [] >>
+metis_tac [infer_p_next_uvar_mono, arithmeticTheory.LESS_EQ_TRANS,
+           pair_CASES,
+           DECIDE ``!(x:num) y. x ≤ x + y``,
+           DECIDE ``!(x:num) y. x + 1 ≤ y ⇒ x ≤ y``,
+           DECIDE ``!(x:num) y z. x ≤ y ⇒ x ≤ y + z``]);
+
+           (*
 val infer_e_sound = Q.prove (
 `(!menv cenv env e st st' ext tenv t.
     (infer_e menv cenv env e st = (Success t, st')) ∧
@@ -140,10 +358,11 @@ val infer_e_sound = Q.prove (
     ?env'. type_funs (convert_menv menv) cenv tenv funs env')`,
 
 ho_match_mp_tac infer_e_ind >>
-rw [infer_e_def, st_ex_return_def, st_ex_bind_success, failwith_def] >>
+rw [infer_e_def, success_eqns, remove_pair_lem] >>
+rw [check_t_def] >>
+fs [bind_def, check_env_def, check_t_def] >>
 ONCE_REWRITE_TAC [type_e_cases] >>
 rw [apply_subst_t_eqn, convert_t_def, Tbool_def, Tint_def, Tunit_def] >|
-
 [fs [fresh_uvar_success] >>
      rw [apply_subst_t_eqn, convert_t_def] >>
      fs [infer_invariant_def, sub_ext_def, LET_THM, FLOOKUP_FUNION] >>
@@ -151,7 +370,44 @@ rw [apply_subst_t_eqn, convert_t_def, Tbool_def, Tint_def, Tunit_def] >|
      rw [convert_t_def] >>
      fs [flookup_thm, count_add1, FRANGE_DEF, SUBSET_DEF] >>
      metis_tac [IN_INSERT, check_convert_freevars, prim_recTheory.LESS_REFL],
+ all_tac,
+ all_tac,
+ all_tac,
+ all_tac,
+ all_tac,
+ all_tac,
+ (* Opref *)
+     rw [typeSystemTheory.type_uop_cases, Tref_def] >>
+     metis_tac [],
+ (* Opderef *)
+ (*
+     `sub_ext (count st''.next_uvar) (num_tvs some_tenv) st''.subst some_ext` by cheat >>
+     `tenv_rel (st''.subst ⊌ some_ext) env some_tenv` by cheat >>
+     `
+     rw [typeSystemTheory.type_uop_cases, Tref_def] >>
+     *)
+     
+ all_tac,
+ all_tac,
+ all_tac,
+ all_tac,
+ all_tac,
+ all_tac,
+ all_tac,
+ all_tac,
+ all_tac,
+ all_tac,
+ all_tac,
+ all_tac,
+ all_tac,
+ all_tac,
+ all_tac,
+ all_tac,
+ all_tac,
+ all_tac]
+ *)
 
+ (*
 (* Fn case *)
 rw [Tfn_def]
  
